src/Exp.v
@@ -5,6 +5,8 @@ Require Export
 From Equations Require Import Equations.
 Set Equations With UIP.
 
+Generalizable All Variables.
+
 Section Exp.
 
 Import ListNotations.
@@ -93,6 +95,41 @@ Inductive ValueP Γ : ∀ {τ}, Exp Γ τ → Type :=
   | LambdaP {dom cod} (e : Exp (dom :: Γ) cod) : ValueP Γ (LAM Γ e).
 
 Derive Signature for ValueP.
+
+Lemma ValueP_irrelevance {Γ τ} (v : Exp Γ τ) (H1 H2 : ValueP _ v) :
+  H1 = H2.
+Proof.
+  induction H1; dependent elimination H2; auto.
+  - now erewrite IHValueP1, IHValueP2; eauto.
+  - now erewrite IHValueP1, IHValueP2; eauto.
+Qed.
+
+Inductive Value : Ty → Type :=
+  | HostValue {ty}         : HostExp (TyHost ty) → Value (TyHost ty)
+  | VUnit                  : Value TyUnit
+  | VTrue                  : Value TyBool
+  | VFalse                 : Value TyBool
+  | VPair {τ1 τ2}          : Value τ1 → Value τ2 → Value (TyPair τ1 τ2)
+  | VNil {τ}               : Value (TyList τ)
+  | VCons {τ}              : Value τ → Value (TyList τ) → Value (TyList τ)
+  | ClosureExp {dom cod}   : Closure dom cod → Value (dom ⟶ cod)
+
+with Closure : Ty → Ty → Type :=
+  | Lambda {dom cod}   : Exp [dom] cod → Closure dom cod
+  | Func {dom cod}     : HostExp (dom ⟶ cod) → Closure dom cod.
+
+Derive Signature NoConfusion for Value.
+Derive Signature NoConfusion Subterm for Closure.
+
+Inductive ValEnv : Env → Type :=
+  | Empty : ValEnv []
+  | Val {Γ τ} : Value τ → ValEnv Γ → ValEnv (τ :: Γ).
+
+Derive Signature NoConfusion for ValEnv.
+
+Equations get_value `(s : ValEnv Γ) `(v : Var Γ τ) : Value τ :=
+  get_value (Val x _)  (ZV _ _)     := x;
+  get_value (Val _ xs) (SV _ _ _ v) := get_value xs v.
 
 End Exp.
 
